Veir/Verifier.lean
@@ -538,6 +538,47 @@ def OperationPtr.verifyLocalInvariants (op : OperationPtr) (ctx : IRContext OpCo
     if op.getNumSuccessors ctx opIn ≠ 0 then
       throw "Expected 0 successors"
     pure ()
+  /- MOD_ARITH -/
+  | .mod_arith_add => do
+    if op.getNumOperands ctx opIn ≠ 2 then
+      throw "Expected 2 operands"
+    if op.getNumResults ctx opIn ≠ 1 then
+      throw "Expected 1 result"
+    if op.getNumRegions ctx opIn ≠ 0 then
+      throw "Expected 0 regions"
+    if op.getNumSuccessors ctx opIn ≠ 0 then
+      throw "Expected 0 successors"
+    pure ()
+  | .mod_arith_constant => do
+    if op.getNumOperands ctx opIn ≠ 0 then
+      throw "Expected 0 operands"
+    if op.getNumResults ctx opIn ≠ 1 then
+      throw "Expected 1 result"
+    if op.getNumRegions ctx opIn ≠ 0 then
+      throw "Expected 0 regions"
+    if op.getNumSuccessors ctx opIn ≠ 0 then
+      throw "Expected 0 successors"
+    pure ()
+  | .mod_arith_mul => do
+    if op.getNumOperands ctx opIn ≠ 2 then
+      throw "Expected 2 operands"
+    if op.getNumResults ctx opIn ≠ 1 then
+      throw "Expected 1 result"
+    if op.getNumRegions ctx opIn ≠ 0 then
+      throw "Expected 0 regions"
+    if op.getNumSuccessors ctx opIn ≠ 0 then
+      throw "Expected 0 successors"
+    pure ()
+  | .mod_arith_sub => do
+    if op.getNumOperands ctx opIn ≠ 2 then
+      throw "Expected 2 operands"
+    if op.getNumResults ctx opIn ≠ 1 then
+      throw "Expected 1 result"
+    if op.getNumRegions ctx opIn ≠ 0 then
+      throw "Expected 0 regions"
+    if op.getNumSuccessors ctx opIn ≠ 0 then
+      throw "Expected 0 successors"
+    pure ()
   /- RISCV -/
   | .riscv_li => do
     if op.getNumOperands ctx opIn ≠ 0 then
