Test/ModArith/identity.mlir
@@ -1,0 +1,20 @@
+// RUN: veir-opt %s | filecheck %s
+
+"builtin.module"() ({
+^bb0():
+  %0 = "mod_arith.constant"() <{"value" = 13 : i32}> : () -> !mod_arith.int<17 : i32>
+  %1 = "mod_arith.constant"() <{"value" = 7 : i32}> : () -> !mod_arith.int<17 : i32>
+  %2 = "mod_arith.add"(%0, %1) : (!mod_arith.int<17 : i32>, !mod_arith.int<17 : i32>) -> !mod_arith.int<17 : i32>
+  %3 = "mod_arith.sub"(%0, %1) : (!mod_arith.int<17 : i32>, !mod_arith.int<17 : i32>) -> !mod_arith.int<17 : i32>
+  %4 = "mod_arith.mul"(%0, %1) : (!mod_arith.int<17 : i32>, !mod_arith.int<17 : i32>) -> !mod_arith.int<17 : i32>
+}) : () -> ()
+
+
+// CHECK:       "builtin.module"() ({
+// CHECK-NEXT:   ^4():
+// CHECK-NEXT:     %{{.*}} = "mod_arith.constant"() <{"value" = 13 : i32}> : () -> !mod_arith.int<17 : i32>
+// CHECK-NEXT:     %{{.*}} = "mod_arith.constant"() <{"value" = 7 : i32}> : () -> !mod_arith.int<17 : i32>
+// CHECK-NEXT:     %{{.*}} = "mod_arith.add"(%{{.*}}, %{{.*}}) : (!mod_arith.int<17 : i32>, !mod_arith.int<17 : i32>) -> !mod_arith.int<17 : i32>
+// CHECK-NEXT:     %{{.*}} = "mod_arith.sub"(%{{.*}}, %{{.*}}) : (!mod_arith.int<17 : i32>, !mod_arith.int<17 : i32>) -> !mod_arith.int<17 : i32>
+// CHECK-NEXT:     %{{.*}} = "mod_arith.mul"(%{{.*}}, %{{.*}}) : (!mod_arith.int<17 : i32>, !mod_arith.int<17 : i32>) -> !mod_arith.int<17 : i32>
+// CHECK-NEXT: }) : () -> ()
